Definitions/Semantics.v
@@ -13,166 +13,191 @@ Require Import Coq.Program.Equality.
 Reserved Notation "e '⇓' n" (at level 50, left associativity).
 Inductive BigStep   : (Heap * Env * Rho * Expr) -> (Heap * Val * Phi) -> Prop:=
 | BS_Nat_Cnt :
-  forall n env rho heap,
-    (heap, env, rho, Const n) ⇓ (heap, Num n, Phi_Nil)
+  forall n env rho heap phi,
+    phi = Phi_Nil ->
+    (heap, env, rho, Const n) ⇓ (heap, Num n, phi)
 
 | BS_Boolean :
-  forall b env rho heap,
-    (heap, env, rho, Bool b) ⇓ (heap, Bit b, Phi_Nil)
+  forall b env rho heap phi,
+    phi = Phi_Nil ->
+    (heap, env, rho, Bool b) ⇓ (heap, Bit b, phi)
 
 | BS_Val_Var :
-  forall x v env rho heap,
-    find_E x env = Some v -> (heap, env, rho, Var x) ⇓ (heap, v, Phi_Nil)
+  forall x v env rho heap phi,
+    phi = Phi_Nil ->
+    find_E x env = Some v -> (heap, env, rho, Var x) ⇓ (heap, v, phi)
 
 | BS_Mu_Abs :
-  forall f x ec ee env rho (heap fheap : Heap),
-    (heap, env, rho, Mu f x ec ee) ⇓ (heap, Cls (env, rho, Mu f x ec ee), Phi_Nil)
+  forall f x ec ee env rho (heap fheap : Heap) phi,
+    phi = Phi_Nil ->
+    (heap, env, rho, Mu f x ec ee) ⇓ (heap, Cls (env, rho, Mu f x ec ee), phi)
 
 | BS_Lambda_Abs :
-  forall x eb env rho heap,
-    (heap, env, rho, Lambda x eb) ⇓ (heap, Cls (env, rho, Lambda x eb), Phi_Nil)
+  forall x eb env rho heap phi,
+    phi = Phi_Nil ->
+    (heap, env, rho, Lambda x eb) ⇓ (heap, Cls (env, rho, Lambda x eb), phi)
 
 | BS_Mu_App :
   forall (f : VarId) x ef ea ec' ee' v v'
          (env env': Env) (rho rho' : Rho) (heap fheap aheap bheap : Heap)
-         (facts aacts bacts : Phi),
+         (phi facts aacts bacts : Phi),
     (heap, env, rho, ef) ⇓ (fheap, Cls (env', rho', Mu f x ec' ee'), facts) ->
     (fheap, env, rho, ea) ⇓ (aheap, v, aacts) ->
     (aheap, update_rec_E (f, Cls (env', rho', Mu f x ec' ee')) (x, v) env', rho', ec')
       ⇓ (bheap, v', bacts) ->
-    (heap, env, rho,  Mu_App ef ea) ⇓ (bheap, v', Phi_Seq (Phi_Seq facts aacts) bacts)
+    phi = (Phi_Seq (Phi_Seq facts aacts) bacts) ->
+    (heap, env, rho,  Mu_App ef ea) ⇓ (bheap, v', phi)
 
 | BS_Rgn_App :
   forall x er eb w v v' (env env': Env) (rho rho' : Rho)
-         (heap fheap aheap bheap : Heap) (facts aacts bacts : Phi),
+         (heap fheap aheap bheap : Heap) (phi facts aacts bacts : Phi),
     (heap, env, rho, er) ⇓ (fheap, Cls (env', rho', Lambda x eb), facts) ->
     find_R w rho = Some v' ->
     (fheap, env', update_R (x, v') rho' , eb) ⇓ (bheap, v, bacts) ->
-    (heap, env, rho, Rgn_App er w) ⇓ (bheap, v, Phi_Seq facts bacts)
+    phi = (Phi_Seq facts bacts) ->
+    (heap, env, rho, Rgn_App er w) ⇓ (bheap, v, phi)
 
 | BS_Eff_App :
   forall (f : VarId) x ef ea ec' ee' v v'
-         (env env': Env) (rho rho' : Rho) heap (facts aacts bacts : Phi),
+         (env env': Env) (rho rho' : Rho) heap (phi facts aacts bacts : Phi),
     (heap, env, rho, ef) ⇓ (heap, Cls (env', rho', Mu f x ec' ee'), facts) ->
     (heap, env, rho, ea) ⇓ (heap, v', aacts) ->
     (heap, update_rec_E (f, Cls (env', rho', Mu f x ec' ee')) (x, v') env', rho', ee')
       ⇓ (heap, v, bacts) ->
-    (heap, env, rho, Eff_App ef ea) ⇓ (heap, v, Phi_Seq (Phi_Seq facts aacts) bacts)
+    phi = (Phi_Seq (Phi_Seq facts aacts) bacts) ->
+    (heap, env, rho, Eff_App ef ea) ⇓ (heap, v, phi)
 
 | BS_Pair_Par :
   forall env rho ea1 ef1 ea2 ef2 v1 v2 theta1 theta2
          (heap_eff1 heap_eff2 heap heap_mu1 heap_mu2 heap' : Heap)
-         (acts_mu1 acts_mu2 acts_eff1 acts_eff2 : Phi),
+         (phi acts_mu1 acts_mu2 acts_eff1 acts_eff2 : Phi),
     (heap, env, rho, Eff_App ef1 ea1) ⇓ (heap_eff1, Eff theta1, acts_eff1) ->
     (heap, env, rho, Eff_App ef2 ea2) ⇓ (heap_eff2, Eff theta2, acts_eff2) ->
     Disjointness theta1 theta2 /\ not (Conflictness theta1 theta2) ->
     (heap, env, rho, Mu_App ef1 ea1) ⇓ (heap_mu1, v1, acts_mu1) ->
     (heap, env, rho, Mu_App ef2 ea2) ⇓ (heap_mu2, v2, acts_mu2) ->
     (Phi_Par acts_mu1 acts_mu2, heap) ==>* (Phi_Nil, heap') ->
-    (heap, env, rho, Pair_Par ef1 ea1 ef2 ea2) ⇓ (heap', Pair (v1, v2),
-        Phi_Seq (Phi_Par acts_eff1 acts_eff2) (Phi_Par acts_mu1 acts_mu2))
+    phi = (Phi_Seq (Phi_Par acts_eff1 acts_eff2) (Phi_Par acts_mu1 acts_mu2)) ->
+    (heap, env, rho, Pair_Par ef1 ea1 ef2 ea2) ⇓ (heap', Pair (v1, v2), phi)
 
 | BS_Cond_True :
-  forall e et ef env rho v (heap cheap theap : Heap) (cacts tacts : Phi),
+  forall e et ef env rho v (heap cheap theap : Heap) (phi cacts tacts : Phi),
     (heap, env, rho, e) ⇓ (cheap, (Bit true), cacts) ->
     (cheap, env, rho, et) ⇓ (theap, v, tacts) ->
-    (heap, env, rho, Cond e et ef) ⇓ (theap, v, Phi_Seq cacts tacts)
+    phi = (Phi_Seq cacts tacts) ->
+    (heap, env, rho, Cond e et ef) ⇓ (theap, v, phi)
 
 | BS_Cond_False :
-  forall e et ef env rho v (heap cheap fheap : Heap) (cacts facts : Phi),
+  forall e et ef env rho v (heap cheap fheap : Heap) (phi cacts facts : Phi),
     (heap, env, rho, e) ⇓ (cheap, (Bit false), cacts) ->
     (cheap, env, rho, ef) ⇓ (fheap, v, facts) ->
-    (heap, env, rho, Cond e et ef) ⇓ (fheap, v, Phi_Seq cacts facts)
+    phi = (Phi_Seq cacts facts) ->
+    (heap, env, rho, Cond e et ef) ⇓ (fheap, v, phi)
 
 | BS_New_Ref :
-  forall e w r l v env rho  (heap heap' : Heap) vacts,
+  forall e w r l v env rho  (heap heap' : Heap) (phi vacts : Phi),
     (heap, env, rho, e) ⇓ (heap', v, vacts) ->
     find_R w rho = Some r ->
     (*find_H (r, l) heap' = None -> *)
     allocate_H heap' r = l ->
-    (heap, env, rho, Ref w e) ⇓ (update_H ((r, l), v) heap', Loc (Rgn2_Const true false r) l,
-        Phi_Seq vacts (Phi_Elem (DA_Alloc r l v)))
+    phi = (Phi_Seq vacts (Phi_Elem (DA_Alloc r l v))) ->
+    (heap, env, rho, Ref w e) ⇓
+      (update_H ((r, l), v) heap', Loc (Rgn2_Const true false r) l, phi)
 
-| BS_Get_Ref : forall ea w r l v env rho (heap heap' : Heap) aacts,
+| BS_Get_Ref : forall ea w r l v env rho (heap heap' : Heap) (phi aacts : Phi),
     (heap, env, rho, ea) ⇓ (heap', Loc w l, aacts) ->
     find_R w rho = Some r ->
     find_H (r, l) heap' = Some v ->
-    (heap, env, rho, DeRef w ea) ⇓ (heap', v, Phi_Seq aacts (Phi_Elem (DA_Read r l v)))
+    phi = (Phi_Seq aacts (Phi_Elem (DA_Read r l v))) ->
+    (heap, env, rho, DeRef w ea) ⇓ (heap', v, phi)
 
 | BS_Set_Ref :
-  forall ea ev w r l v env rho (heap heap' heap'' : Heap) (aacts vacts : Phi),
+  forall ea ev w r l v env rho (heap heap' heap'' : Heap) (phi aacts vacts : Phi),
     (heap, env, rho, ea) ⇓ (heap', Loc w l, aacts) ->
     (heap', env, rho, ev) ⇓ (heap'', v, vacts) ->
     find_R w rho = Some r ->
-    (heap, env, rho, Assign w ea ev) ⇓ (update_H ((r, l), v) heap'', Unit,
-        Phi_Seq (Phi_Seq aacts vacts) (Phi_Elem (DA_Write r l v)))
+    phi = Phi_Seq (Phi_Seq aacts vacts) (Phi_Elem (DA_Write r l v)) ->
+    (heap, env, rho, Assign w ea ev) ⇓ (update_H ((r, l), v) heap'', Unit, phi)
 
 | BS_Nat_Plus :
-  forall a b va vb env rho (heap lheap rheap : Heap) (lacts racts : Phi),
+  forall a b va vb env rho (heap lheap rheap : Heap) (phi lacts racts : Phi),
     (heap, env, rho, a) ⇓ (lheap, Num va, lacts) ->
     (lheap, env, rho, b) ⇓ (rheap, Num vb, racts) ->
-    (heap, env, rho, Plus a b) ⇓ (rheap, Num (va + vb), Phi_Seq lacts racts)
+    phi = ( Phi_Seq lacts racts) ->
+    (heap, env, rho, Plus a b) ⇓ (rheap, Num (va + vb), phi)
 
 | BS_Nat_Minus :
-  forall a b va vb env rho (heap lheap rheap : Heap) (lacts racts : Phi),
+  forall a b va vb env rho (heap lheap rheap : Heap) (phi lacts racts : Phi),
     (heap, env, rho, a) ⇓ (lheap, Num va, lacts) ->
     (lheap, env, rho, b) ⇓ (rheap, Num vb, racts) ->
-    (heap, env, rho, Minus a b) ⇓ (rheap, Num (va - vb), Phi_Seq lacts racts)
+     phi = ( Phi_Seq lacts racts) ->
+    (heap, env, rho, Minus a b) ⇓ (rheap, Num (va - vb), phi)
 
 | BS_Nat_Times :
-  forall a b va vb env rho (heap lheap rheap : Heap) (lacts racts : Phi),
+  forall a b va vb env rho (heap lheap rheap : Heap) (phi lacts racts : Phi),
     (heap, env, rho, a) ⇓ (lheap, Num va, lacts) ->
     (lheap, env, rho, b) ⇓ (rheap, Num vb, racts) ->
-    (heap, env, rho, Times a b) ⇓ (rheap, Num (va * vb), Phi_Seq lacts racts)
+    phi = ( Phi_Seq lacts racts) ->
+    (heap, env, rho, Times a b) ⇓ (rheap, Num (va * vb), phi)
 
 | BS_Bool_Eq :
-  forall a b va vb env rho (heap lheap rheap : Heap) (lacts racts : Phi),
+  forall a b va vb env rho (heap lheap rheap : Heap) (phi lacts racts : Phi),
     (heap, env, rho, a) ⇓ (lheap, Num va, lacts) ->
     (lheap, env, rho, b) ⇓ (rheap, Num vb, racts) ->
-    (heap, env, rho, Eq a b) ⇓ (rheap, Bit (Nat.eqb va vb), Phi_Seq lacts racts)
+    phi = ( Phi_Seq lacts racts) ->
+    (heap, env, rho, Eq a b) ⇓ (rheap, Bit (Nat.eqb va vb), phi)
 
 | BS_Alloc_Abs :
-  forall w r env rho heap,
+  forall w r env rho heap phi,
     find_R w rho = Some r ->
-    (heap, env, rho, AllocAbs w) ⇓ (heap, Eff (Some (singleton_set (CA_AllocAbs r))), Phi_Nil)
+    phi = Phi_Nil ->
+    (heap, env, rho, AllocAbs w) ⇓
+      (heap, Eff (Some (singleton_set (CA_AllocAbs r))), phi)
 
 | BS_Read_Abs :
-  forall w r env rho heap,
+  forall w r env rho heap phi,
     find_R w rho = Some r ->
-    (heap, env, rho, ReadAbs w) ⇓ (heap, Eff (Some (singleton_set (CA_ReadAbs r))), Phi_Nil)
+    phi = Phi_Nil ->
+    (heap, env, rho, ReadAbs w) ⇓
+      (heap, Eff (Some (singleton_set (CA_ReadAbs r))), phi)
 
 | BS_Write_Abs :
-  forall w r env rho heap,
+  forall w r env rho heap phi,
     find_R w rho = Some r ->
-    (heap, env, rho, WriteAbs w) ⇓ (heap, Eff (Some (singleton_set (CA_WriteAbs r))), Phi_Nil)
+    phi = Phi_Nil ->
+    (heap, env, rho, WriteAbs w) ⇓
+      (heap, Eff (Some (singleton_set (CA_WriteAbs r))), phi)
 
 | BS_Read_Conc :
-  forall ea r l env rho (heap heap' : Heap) aacts,
-    (heap, env, rho, ea) ⇓ (heap', Loc (Rgn2_Const true false r) l, aacts) ->
-    aacts = Phi_Nil ->
-    (heap, env, rho, ReadConc ea) ⇓ (heap', Eff (Some (singleton_set (CA_ReadConc r l))),
-        Phi_Nil)
+  forall ea r l env rho (heap heap' : Heap) phi,
+    (heap, env, rho, ea) ⇓ (heap', Loc (Rgn2_Const true false r) l, phi) ->
+    phi = Phi_Nil ->
+    (heap, env, rho, ReadConc ea) ⇓
+      (heap', Eff (Some (singleton_set (CA_ReadConc r l))), phi)
 
 | BS_Write_Conc :
-  forall ea r l env rho (heap heap' : Heap) aacts,
-    (heap, env, rho, ea) ⇓ (heap', Loc (Rgn2_Const true false r) l, aacts) ->
-    aacts = Phi_Nil ->
-    (heap, env, rho, WriteConc ea) ⇓ (heap', Eff (Some (singleton_set (CA_WriteConc r l))),
-        Phi_Nil)
+  forall ea r l env rho (heap heap' : Heap) phi,
+    (heap, env, rho, ea) ⇓ (heap', Loc (Rgn2_Const true false r) l, phi) ->
+    phi = Phi_Nil ->
+    (heap, env, rho, WriteConc ea) ⇓
+      (heap', Eff (Some (singleton_set (CA_WriteConc r l))), phi)
 
 | BS_Eff_Concat :
-  forall a b env rho heap (effa effb : Theta) phia phib,
+  forall a b env rho heap (effa effb : Theta) (phi phia phib : Phi),
     (heap, env, rho, a) ⇓ (heap, Eff effa, phia) ->
     (heap, env, rho, b) ⇓ (heap, Eff effb, phib) ->
-    (heap, env, rho, Concat a b) ⇓ (heap, Eff (Union_Theta effa effb), Phi_Seq phia phib)
+    phi = (Phi_Seq phia phib) ->
+    (heap, env, rho, Concat a b) ⇓ (heap, Eff (Union_Theta effa effb), phi)
 
 | BS_Eff_Top :
-  forall env rho heap,
-    (heap, env, rho, Top) ⇓ (heap, Eff None, Phi_Nil)
+  forall env rho heap phi,
+     phi = Phi_Nil ->
+    (heap, env, rho, Top) ⇓ (heap, Eff None, phi)
 
 | BS_Eff_Empty :
-  forall  env rho heap,
-    (heap, env, rho, Empty) ⇓ (heap, Eff (Some empty_set), Phi_Nil)    
+  forall  env rho heap phi,
+     phi = Phi_Nil ->
+    (heap, env, rho, Empty) ⇓ (heap, Eff (Some empty_set), phi)    
 where "e '⇓' n" := (BigStep e n) : type_scope.
 
 Tactic Notation "dynamic_cases" tactic (first) ident(c) :=
